theories/coneris/examples/hash/con_hash_interface0.v
@@ -1,0 +1,61 @@
+From clutch.coneris Require Import coneris .
+
+Set Default Proof Using "Type*".
+
+Class con_hash0 `{!conerisGS Σ} (val_size:nat):= Con_Hash0
+{
+  (** * Operations *)
+  init_hash0 : val;
+  (* incr_counter : val; *)
+  allocate_tape0 : val;
+  compute_hash0 : val;
+  (** * Ghost state *)
+  
+  (** [name] is used to associate [locked] with [is_lock] *)
+  (* tape_name: Type; *)
+  
+  hash_view_gname:Type;
+  hash_map_gname:Type;
+  hash_lock_gname:Type;
+  
+  (** * Predicates *)
+  con_hash_inv0  (f l hm: val) (γ1:hash_view_gname) (γ2:hash_map_gname) (γ_lock:hash_lock_gname): iProp Σ;
+  (* concrete_seq_hash {L:seq_hashG Σ} (f:val) (m:gmap nat nat) : iProp Σ;  *)
+  hash_tape0 (α:val) (ns:list nat) : iProp Σ;
+  con_hash_view0 (v res:nat) (γ:hash_view_gname): iProp Σ;
+  
+  (** * General properties of the predicates *)
+  (* #[global] concrete_seq_hash_timeless {L : seq_hashG Σ} f m :: *)
+  (*   Timeless (concrete_seq_hash (L:=L) f m); *)
+  #[global] hash_tape_timeless α ns ::
+    Timeless (hash_tape0 α ns); 
+  #[global] con_hash_view_timeless v res γ ::
+    Timeless (con_hash_view0 v res γ);
+  con_hash_view_frag_frag_agree k v1 v2 γ :
+    con_hash_view0 k v1 γ -∗ con_hash_view0 k v2 γ -∗ ⌜v1=v2⌝; 
+
+  con_hash_presample0 E (ε:nonnegreal) ns α (ε2 : fin (S val_size) → R) :
+    (∀ x : fin (S val_size), (0 <= ε2 x)%R)->
+    (SeriesC (λ n : fin (S val_size), 1 / S val_size * ε2 n) <= ε)%R ->
+    hash_tape0 α ns -∗
+    ↯ ε -∗
+    state_update E E (∃ n,
+          ↯ (ε2 n) ∗
+          hash_tape0 α (ns++[fin_to_nat n]) 
+      );
+  con_hash_spec0 f l hm γ1 γ2 γlock α n ns (v:nat):
+    {{{ con_hash_inv0 f l hm γ1 γ2 γlock ∗ hash_tape0 α (n::ns) }}}
+      f #v α
+      {{{ (res:nat), RET (#res);  con_hash_view0 v res γ1 ∗
+                                (hash_tape0 α ns ∗ ⌜res=n⌝ ∨
+                                 hash_tape0 α (n::ns)
+                                )
+      }}};
+  con_hash_spec_hashed_before0 f l hm γ1 γ2 γlock α ns res (v:nat):
+    {{{ con_hash_inv0 f l hm γ1 γ2 γlock ∗ hash_tape0 α ns ∗ con_hash_view0 v res γ1}}}
+      f #v α
+      {{{ RET (#res);  con_hash_view0 v res γ1 ∗
+                       (hash_tape0 α ns)
+      }}}
+}.
+
